FormalWeb/TransitionTrace.lean
@@ -1,0 +1,41 @@
+namespace FormalWeb
+
+inductive TransitionTrace
+    (stepFn : σ → α → Option σ) :
+    σ → List α → σ → Prop where
+  | nil (state : σ) : TransitionTrace stepFn state [] state
+  | cons
+      {start intermediate finish : σ}
+      {action : α}
+      {actions : List α} :
+      stepFn start action = some intermediate →
+      TransitionTrace stepFn intermediate actions finish →
+      TransitionTrace stepFn start (action :: actions) finish
+
+namespace TransitionTrace
+
+theorem single
+    {stepFn : σ → α → Option σ}
+    {start finish : σ}
+    {action : α}
+    (h : stepFn start action = some finish) :
+    TransitionTrace stepFn start [action] finish :=
+  .cons h (.nil finish)
+
+theorem append
+    {stepFn : σ → α → Option σ}
+    {start middle finish : σ}
+    {xs ys : List α}
+    (hxs : TransitionTrace stepFn start xs middle)
+    (hys : TransitionTrace stepFn middle ys finish) :
+    TransitionTrace stepFn start (xs ++ ys) finish := by
+  induction hxs with
+  | nil state =>
+      simpa using hys
+  | @cons start intermediate finish action actions hstep htrace ih =>
+      simp
+      exact TransitionTrace.cons hstep (ih hys)
+
+end TransitionTrace
+
+end FormalWeb
